Base Dead Code Elim on Subst01
Based on https://github.com/coq/coq/issues/8993#issuecomment-438572277,
I am guessing that DCE is currently memory-hungry.  This makes sense,
because every [var] is carrying around a full `PositiveSet.t` when
computing live variables.  Instead, we now adjust `subst01` to not
increment counts coming from dead variables, and use it to implement
DCE.  Hopefully this will be much faster and more efficient.

N.B. It was important to stop doing union of `PositiveMap.t`, and
instead add to them incrementally.

Before: p384_32.c (real: 406.78, user: 391.99, sys: 14.82, mem: 16896040 ko)
After:  p384_32.c (real: 201.11, user: 200.33, sys:  0.80, mem:  1039520 ko)

After     | File Name                                                            | Before    || Change    | % Change
--------------------------------------------------------------------------------------------------------------------
21m16.47s | Total                                                                | 24m45.69s || -3m29.22s | -14.08%
--------------------------------------------------------------------------------------------------------------------
3m20.33s  | p384_32.c                                                            | 6m31.99s  || -3m11.66s | -48.89%
0m14.08s  | secp256k1_32.c                                                       | 0m18.85s  || -0m04.77s | -25.30%
0m13.86s  | p256_32.c                                                            | 0m18.14s  || -0m04.28s | -23.59%
6m14.92s  | Experiments/NewPipeline/SlowPrimeSynthesisExamples.vo                | 6m17.66s  || -0m02.74s | -0.72%
4m37.51s  | Experiments/NewPipeline/Toplevel1.vo                                 | 4m39.20s  || -0m01.68s | -0.60%
0m06.46s  | p224_32.c                                                            | 0m07.85s  || -0m01.38s | -17.70%
0m02.49s  | Experiments/NewPipeline/MiscCompilerPassesProofs.vo                  | 0m03.85s  || -0m01.35s | -35.32%
1m32.10s  | Experiments/NewPipeline/Toplevel2.vo                                 | 1m31.75s  || +0m00.34s | +0.38%
0m42.06s  | Experiments/NewPipeline/ExtractionOCaml/word_by_word_montgomery      | 0m42.17s  || -0m00.10s | -0.26%
0m39.54s  | p521_32.c                                                            | 0m39.37s  || +0m00.17s | +0.43%
0m39.45s  | Experiments/NewPipeline/ExtractionHaskell/word_by_word_montgomery    | 0m39.51s  || -0m00.05s | -0.15%
0m32.87s  | p521_64.c                                                            | 0m32.94s  || -0m00.07s | -0.21%
0m25.29s  | Experiments/NewPipeline/ExtractionHaskell/unsaturated_solinas        | 0m25.26s  || +0m00.02s | +0.11%
0m23.06s  | Experiments/NewPipeline/ExtractionOCaml/unsaturated_solinas          | 0m23.20s  || -0m00.14s | -0.60%
0m18.73s  | Experiments/NewPipeline/ExtractionHaskell/saturated_solinas          | 0m19.01s  || -0m00.28s | -1.47%
0m14.93s  | Experiments/NewPipeline/ExtractionOCaml/saturated_solinas            | 0m15.04s  || -0m00.10s | -0.73%
0m10.58s  | p384_64.c                                                            | 0m11.21s  || -0m00.63s | -5.61%
0m09.12s  | Experiments/NewPipeline/ExtractionOCaml/word_by_word_montgomery.ml   | 0m08.90s  || +0m00.21s | +2.47%
0m05.94s  | Experiments/NewPipeline/ExtractionOCaml/unsaturated_solinas.ml       | 0m06.06s  || -0m00.11s | -1.98%
0m05.78s  | Experiments/NewPipeline/ExtractionHaskell/word_by_word_montgomery.hs | 0m05.76s  || +0m00.02s | +0.34%
0m04.36s  | Experiments/NewPipeline/ExtractionOCaml/saturated_solinas.ml         | 0m04.37s  || -0m00.00s | -0.22%
0m04.23s  | Experiments/NewPipeline/ExtractionHaskell/unsaturated_solinas.hs     | 0m04.24s  || -0m00.00s | -0.23%
0m03.47s  | Experiments/NewPipeline/ExtractionHaskell/saturated_solinas.hs       | 0m03.68s  || -0m00.20s | -5.70%
0m02.38s  | curve25519_32.c                                                      | 0m02.39s  || -0m00.01s | -0.41%
0m02.04s  | secp256k1_64.c                                                       | 0m02.09s  || -0m00.04s | -2.39%
0m01.94s  | p224_64.c                                                            | 0m01.96s  || -0m00.02s | -1.02%
0m01.90s  | p256_64.c                                                            | 0m01.96s  || -0m00.06s | -3.06%
0m01.52s  | curve25519_64.c                                                      | 0m01.60s  || -0m00.08s | -5.00%
0m01.47s  | Experiments/NewPipeline/CLI.vo                                       | 0m01.44s  || +0m00.03s | +2.08%
0m01.22s  | Experiments/NewPipeline/StandaloneHaskellMain.vo                     | 0m01.26s  || -0m00.04s | -3.17%
0m01.21s  | Experiments/NewPipeline/StandaloneOCamlMain.vo                       | 0m01.27s  || -0m00.06s | -4.72%
0m00.97s  | Experiments/NewPipeline/CompilersTestCases.vo                        | 0m01.10s  || -0m00.13s | -11.81%
0m00.66s  | Experiments/NewPipeline/MiscCompilerPasses.vo                        | 0m00.62s  || +0m00.04s | +6.45%

src/Experiments/NewPipeline/MiscCompilerPasses.v
@@ -11,137 +11,108 @@ Module Compilers.
   Import invert_expr.
   Import defaults.
 
+  Module Subst01.
+    Section with_counter.
+      Context {t : Type}
+              (one : t)
+              (incr : t -> t).
+
+      Local Notation PositiveMap_incr idx m
+        := (PositiveMap.add idx (match PositiveMap.find idx m with
+                                 | Some n => incr n
+                                 | None => one
+                                 end) m).
+
+      Section with_ident.
+        Context {base_type : Type}.
+        Local Notation type := (type.type base_type).
+        Context {ident : type -> Type}.
+        Local Notation expr := (@expr.expr base_type ident).
+        (** N.B. This does not work well when let-binders are not at top-level *)
+        Fixpoint compute_live_counts' {t} (e : @expr (fun _ => positive) t) (cur_idx : positive) (live : PositiveMap.t _)
+          : positive * PositiveMap.t _
+          := match e with
+             | expr.Var t v => (cur_idx, PositiveMap_incr v live)
+             | expr.Ident t idc => (cur_idx, live)
+             | expr.App s d f x
+               => let '(idx, live) := @compute_live_counts' _ f cur_idx live in
+                  let '(idx, live) := @compute_live_counts' _ x idx live in
+                  (idx, live)
+             | expr.Abs s d f
+               => let '(idx, live) := @compute_live_counts' _ (f cur_idx) (Pos.succ cur_idx) live in
+                  (cur_idx, live)
+             | expr.LetIn tx tC ex eC
+               => let '(idx, live) := @compute_live_counts' tC (eC cur_idx) (Pos.succ cur_idx) live in
+                  if PositiveMap.mem cur_idx live
+                  then @compute_live_counts' tx ex idx live
+                  else (idx, live)
+             end.
+        Definition compute_live_counts {t} e : PositiveMap.t _ := snd (@compute_live_counts' t e 1 (PositiveMap.empty _)).
+        Definition ComputeLiveCounts {t} (e : expr.Expr t) := compute_live_counts (e _).
+
+        Section with_var.
+          Context (doing_subst : forall T1 T2, T1 -> T2 -> T1)
+                  {var : type -> Type}
+                  (should_subst : t -> bool)
+                  (live : PositiveMap.t t).
+          Fixpoint subst0n' {t} (e : @expr (@expr var) t) (cur_idx : positive)
+            : positive * @expr var t
+            := match e with
+               | expr.Var t v => (cur_idx, v)
+               | expr.Ident t idc => (cur_idx, expr.Ident idc)
+               | expr.App s d f x
+                 => let '(idx, f') := @subst0n' _ f cur_idx in
+                    let '(idx, x') := @subst0n' _ x idx in
+                    (idx, expr.App f' x')
+               | expr.Abs s d f
+                 => (cur_idx, expr.Abs (fun v => snd (@subst0n' _ (f (expr.Var v)) (Pos.succ cur_idx))))
+               | expr.LetIn tx tC ex eC
+                 => let '(idx, ex') := @subst0n' tx ex cur_idx in
+                    let eC' := fun v => snd (@subst0n' tC (eC v) (Pos.succ cur_idx)) in
+                    if match PositiveMap.find cur_idx live with
+                       | Some n => should_subst n
+                       | None => true
+                       end
+                    then (Pos.succ cur_idx, eC' (doing_subst _ _ ex' (Pos.succ cur_idx, PositiveMap.elements live)))
+                    else (Pos.succ cur_idx, expr.LetIn ex' (fun v => eC' (expr.Var v)))
+               end.
+
+          Definition subst0n {t} e : expr t
+            := snd (@subst0n' t e 1).
+        End with_var.
+
+        Definition Subst0n (doing_subst : forall T1 T2, T1 -> T2 -> T1) (should_subst : t -> bool) {t} (e : expr.Expr t) : expr.Expr t
+          := fun var => subst0n doing_subst should_subst (ComputeLiveCounts e) (e _).
+      End with_ident.
+    End with_counter.
+
+    Section for_01.
+      Inductive one_or_more := one | more.
+      Local Notation t := one_or_more.
+      Let incr : t -> t := fun _ => more.
+      Let should_subst : t -> bool
+        := fun v => match v with
+                    | one => true
+                    | more => false
+                    end.
+
+      Definition Subst01 {base_type ident} {t} (e : expr.Expr t) : expr.Expr t
+        := @Subst0n _ one incr base_type ident (fun _ _ x _ => x) should_subst t e.
+    End for_01.
+  End Subst01.
+
   Module DeadCodeElimination.
     Section with_ident.
       Context {base_type : Type}.
       Local Notation type := (type.type base_type).
       Context {ident : type -> Type}.
       Local Notation expr := (@expr.expr base_type ident).
-      Fixpoint compute_live' {t} (e : @expr (fun _ => PositiveSet.t) t) (cur_idx : positive)
-        : positive * PositiveSet.t
-        := match e with
-           | expr.Var t v => (cur_idx, v)
-           | expr.App s d f x
-             => let '(idx, live1) := @compute_live' _ f cur_idx in
-                let '(idx, live2) := @compute_live' _ x idx in
-                (idx, PositiveSet.union live1 live2)
-           | expr.Abs s d f
-             => let '(_, live) := @compute_live' _ (f PositiveSet.empty) cur_idx in
-                (cur_idx, live)
-           | expr.LetIn tx tC ex eC
-             => let '(idx, live) := @compute_live' tx ex cur_idx in
-                let '(_, live) := @compute_live' tC (eC (PositiveSet.add idx live)) (Pos.succ idx) in
-                (Pos.succ idx, live)
-           | expr.Ident t idc => (cur_idx, PositiveSet.empty)
-           end.
-      Definition compute_live {t} e : PositiveSet.t := snd (@compute_live' t e 1).
-      Definition ComputeLive {t} (e : expr.Expr t) := compute_live (e _).
 
-      Section with_var.
-        Context {var : type -> Type}
-                (live : PositiveSet.t).
-        Definition OUGHT_TO_BE_UNUSED {T1 T2} (v : T1) (v' : T2) := v.
-        Global Opaque OUGHT_TO_BE_UNUSED.
-        Fixpoint eliminate_dead' {t} (e : @expr (@expr var) t) (cur_idx : positive)
-          : positive * @expr var t
-          := match e with
-             | expr.Var t v => (cur_idx, v)
-             | expr.Ident t idc => (cur_idx, expr.Ident idc)
-             | expr.App s d f x
-               => let '(idx, f') := @eliminate_dead' _ f cur_idx in
-                  let '(idx, x') := @eliminate_dead' _ x idx in
-                  (idx, expr.App f' x')
-             | expr.Abs s d f
-               => (cur_idx, expr.Abs (fun v => snd (@eliminate_dead' _ (f (expr.Var v)) cur_idx)))
-             | expr.LetIn tx tC ex eC
-               => let '(idx, ex') := @eliminate_dead' tx ex cur_idx in
-                  let eC' := fun v => snd (@eliminate_dead' _ (eC v) (Pos.succ idx)) in
-                  if PositiveSet.mem idx live
-                  then (Pos.succ idx, expr.LetIn ex' (fun v => eC' (expr.Var v)))
-                  else (Pos.succ idx, eC' (OUGHT_TO_BE_UNUSED ex' (Pos.succ idx, PositiveSet.elements live)))
-             end.
-
-        Definition eliminate_dead {t} e : expr t
-          := snd (@eliminate_dead' t e 1).
-      End with_var.
+      Definition OUGHT_TO_BE_UNUSED {T1 T2} (v : T1) (v' : T2) := v.
+      Global Opaque OUGHT_TO_BE_UNUSED.
 
       Definition EliminateDead {t} (e : expr.Expr t) : expr.Expr t
-        := fun var => eliminate_dead (ComputeLive e) (e _).
+        := @Subst01.Subst0n unit tt (fun _ => tt) base_type ident (@OUGHT_TO_BE_UNUSED) (fun _ => false) t e.
     End with_ident.
   End DeadCodeElimination.
-
-  Module Subst01.
-    Local Notation PositiveMap_incr idx m
-      := (PositiveMap.add idx (match PositiveMap.find idx m with
-                               | Some n => S n
-                               | None => S O
-                               end) m).
-    Local Notation PositiveMap_union m1 m2
-      := (PositiveMap.map2
-            (fun c1 c2
-             => match c1, c2 with
-                | Some n1, Some n2 => Some (n1 + n2)%nat
-                | Some n, None
-                | None, Some n
-                  => Some n
-                | None, None => None
-                end) m1 m2).
-    Section with_ident.
-      Context {base_type : Type}.
-      Local Notation type := (type.type base_type).
-      Context {ident : type -> Type}.
-      Local Notation expr := (@expr.expr base_type ident).
-      Fixpoint compute_live_counts' {t} (e : @expr (fun _ => positive) t) (cur_idx : positive)
-        : positive * PositiveMap.t nat
-        := match e with
-           | expr.Var t v => (cur_idx, PositiveMap_incr v (PositiveMap.empty _))
-           | expr.Ident t idc => (cur_idx, PositiveMap.empty _)
-           | expr.App s d f x
-             => let '(idx, live1) := @compute_live_counts' _ f cur_idx in
-                let '(idx, live2) := @compute_live_counts' _ x idx in
-                (idx, PositiveMap_union live1 live2)
-           | expr.Abs s d f
-             => let '(idx, live) := @compute_live_counts' _ (f cur_idx) (Pos.succ cur_idx) in
-                (cur_idx, live)
-           | expr.LetIn tx tC ex eC
-             => let '(idx, live1) := @compute_live_counts' tx ex cur_idx in
-                let '(idx, live2) := @compute_live_counts' tC (eC idx) (Pos.succ idx) in
-                (idx, PositiveMap_union live1 live2)
-           end.
-      Definition compute_live_counts {t} e : PositiveMap.t _ := snd (@compute_live_counts' t e 1).
-      Definition ComputeLiveCounts {t} (e : expr.Expr t) := compute_live_counts (e _).
-
-      Section with_var.
-        Context {var : type -> Type}
-                (live : PositiveMap.t nat).
-        Fixpoint subst01' {t} (e : @expr (@expr var) t) (cur_idx : positive)
-          : positive * @expr var t
-          := match e with
-             | expr.Var t v => (cur_idx, v)
-             | expr.Ident t idc => (cur_idx, expr.Ident idc)
-             | expr.App s d f x
-               => let '(idx, f') := @subst01' _ f cur_idx in
-                  let '(idx, x') := @subst01' _ x idx in
-                  (idx, expr.App f' x')
-             | expr.Abs s d f
-               => (cur_idx, expr.Abs (fun v => snd (@subst01' _ (f (expr.Var v)) (Pos.succ cur_idx))))
-             | expr.LetIn tx tC ex eC
-               => let '(idx, ex') := @subst01' tx ex cur_idx in
-                  let eC' := fun v => snd (@subst01' tC (eC v) (Pos.succ idx)) in
-                  if match PositiveMap.find idx live with
-                     | Some n => (n <=? 1)%nat
-                     | None => true
-                     end
-                  then (Pos.succ idx, eC' ex')
-                  else (Pos.succ idx, expr.LetIn ex' (fun v => eC' (expr.Var v)))
-             end.
-
-        Definition subst01 {t} e : expr t
-          := snd (@subst01' t e 1).
-      End with_var.
-
-      Definition Subst01 {t} (e : expr.Expr t) : expr.Expr t
-        := fun var => subst01 (ComputeLiveCounts e) (e _).
-    End with_ident.
-  End Subst01.
 End Compilers.
